src/lowparse/pulse/LowParse.PulseParse.VCList.fst
@@ -17,6 +17,7 @@ module LPS = LowParse.Pulse.Base
 module PPB = LowParse.PulseParse.Base
 module PPC = LowParse.PulseParse.Combinators
 module LPV = LowParse.Pulse.VCList
+module U32 = FStar.UInt32
 
 (* pts_to_parsed for nlist 1: convert between pts_to_parsed p and pts_to_parsed (parse_nlist 1 p) *)
 
@@ -268,3 +269,116 @@ ensures exists* v' .
   Trade.elim_hyp_l _ _ _;
   tl
 }
+
+(* Validator combinators *)
+
+let parse_consume (#k: parser_kind) (#t: Type) (p: parser k t) (b: bytes)
+: GTot (option nat)
+= match parse p b with
+  | Some (_, consumed) -> Some consumed
+  | None -> None
+
+inline_for_extraction
+fn validate_nlist
+  (n: SZ.t)
+  (#k: parser_kind)
+  (#t: Type0)
+  (#p: parser k t)
+  (v: LPS.validator p)
+: LPS.validator #(nlist (SZ.v n) t) #(parse_nlist_kind (SZ.v n) k) (parse_nlist (SZ.v n) p)
+=
+  (input: slice byte)
+  (poffset: R.ref SZ.t)
+  (#offset: Ghost.erased SZ.t)
+  (#pm: perm)
+  (#v_bytes: Ghost.erased bytes)
+{
+  pts_to_len input;
+  let mut pcontinue = true;
+  let mut pcount = n;
+  while (
+    let c = !pcontinue;
+    let r = !pcount;
+    (c && SZ.gt r 0sz)
+  ) invariant exists* c r off .
+    R.pts_to pcontinue c **
+    R.pts_to pcount r **
+    R.pts_to poffset off **
+    pts_to input #pm v_bytes **
+    pure (
+      SZ.v off <= Seq.length v_bytes /\
+      SZ.v r <= SZ.v n /\ (
+      let s0 = Seq.slice v_bytes (SZ.v offset) (Seq.length v_bytes) in
+      let s = Seq.slice v_bytes (SZ.v off) (Seq.length v_bytes) in
+      Some? (parse (parse_nlist (SZ.v n) p) s0) == (c && Some? (parse (parse_nlist (SZ.v r) p) s)) /\
+      (Some? (parse (parse_nlist (SZ.v n) p) s0) ==>
+        (SZ.v offset + snd (Some?.v (parse (parse_nlist (SZ.v n) p) s0)) ==
+         SZ.v off + snd (Some?.v (parse (parse_nlist (SZ.v r) p) s))))
+    ))
+  {
+    let off = !poffset;
+    let r = !pcount;
+    parse_nlist_eq (SZ.v r) p (Seq.slice v_bytes (SZ.v off) (Seq.length v_bytes));
+    let is_valid = v input poffset;
+    if is_valid {
+      pcount := SZ.sub r 1sz
+    } else {
+      pcontinue := false
+    }
+  };
+  let c = !pcontinue;
+  if c {
+    let off = !poffset;
+    parse_nlist_eq 0 p (Seq.slice v_bytes (SZ.v off) (Seq.length v_bytes));
+    true
+  } else {
+    false
+  }
+}
+
+#push-options "--z3rlimit 32"
+
+inline_for_extraction
+fn validate_vclist
+  (min: U32.t)
+  (max: U32.t { U32.v min <= U32.v max } )
+  (#lk: parser_kind)
+  (#lp: parser lk U32.t)
+  (lv: LPS.validator lp)
+  (lr: PPB.leaf_reader lp)
+  (#k: parser_kind)
+  (#t: Type0)
+  (#p: parser k t)
+  (w: LPS.validator p)
+  (u: squash (lk.parser_kind_subkind == Some ParserStrong /\ FStar.SizeT.fits_u64))
+: LPS.validator #(vlarray t (U32.v min) (U32.v max)) #(parse_vclist_kind (U32.v min) (U32.v max) lk k) (parse_vclist (U32.v min) (U32.v max) lp p)
+=
+  (input: slice byte)
+  (poffset: R.ref SZ.t)
+  (#offset: Ghost.erased SZ.t)
+  (#pm: perm)
+  (#v_bytes: Ghost.erased bytes)
+{
+  let sinput = Ghost.hide (Seq.slice v_bytes (SZ.v offset) (Seq.length v_bytes));
+  parse_vclist_eq (U32.v min) (U32.v max) lp p sinput;
+  let offset_val = !poffset;
+  let is_valid_len = lv input poffset;
+  if is_valid_len {
+    let off = !poffset;
+    let count = PPB.read_parsed_from_validator_success lr input offset_val off;
+    if (U32.lt count min || U32.lt max count) {
+      false
+    } else {
+      SZ.fits_u64_implies_fits_32 ();
+      let n = SZ.uint32_to_sizet count;
+      let consumed_n = Ghost.hide (SZ.v off - SZ.v offset);
+      Seq.lemma_eq_elim
+        (Seq.slice sinput consumed_n (Seq.length sinput))
+        (Seq.slice v_bytes (SZ.v off) (Seq.length v_bytes));
+      validate_nlist n w input poffset
+    }
+  } else {
+    false
+  }
+}
+#pop-options
