src/lowparse/pulse/LowParse.PulseParse.FLData.fst
@@ -1,0 +1,72 @@
+module LowParse.PulseParse.FLData
+#lang-pulse
+include LowParse.Spec.FLData
+open FStar.Tactics.V2
+open Pulse.Lib.Pervasives open Pulse.Lib.Slice.Util open Pulse.Lib.Trade
+open Pulse.Lib.Slice
+open LowParse.Spec.Base
+
+module SZ = FStar.SizeT
+module R = Pulse.Lib.Reference
+module Trade = Pulse.Lib.Trade.Util
+module S = Pulse.Lib.Slice
+module LPS = LowParse.Pulse.Base
+
+inline_for_extraction
+fn validate_fldata
+  (#k: parser_kind)
+  (#t: Type0)
+  (#p: parser k t)
+  (v: LPS.validator p)
+  (sz: SZ.t)
+: LPS.validator #t #(parse_fldata_kind (SZ.v sz) k) (parse_fldata p (SZ.v sz))
+=
+  (input: slice byte)
+  (poffset: R.ref SZ.t)
+  (#offset: Ghost.erased SZ.t)
+  (#pm: perm)
+  (#v_bytes: Ghost.erased bytes)
+{
+  pts_to_len input;
+  let offset_val = !poffset;
+  let remaining = SZ.sub (len input) offset_val;
+  if SZ.lt remaining sz {
+    false
+  } else {
+    let split_point = SZ.add offset_val sz;
+    let input1, input2 = split_trade input split_point;
+    with v2 . assert (pts_to input2 #pm v2);
+    Trade.elim_hyp_r (pts_to input1 #pm _) (pts_to input2 #pm v2) (pts_to input #pm v_bytes);
+    let is_valid = v input1 poffset;
+    if is_valid {
+      let off = !poffset;
+      Trade.elim (pts_to input1 #pm _) (pts_to input #pm v_bytes);
+      if (off = split_point) {
+        true
+      } else {
+        false
+      }
+    } else {
+      Trade.elim (pts_to input1 #pm _) (pts_to input #pm v_bytes);
+      false
+    }
+  }
+}
+
+inline_for_extraction
+fn jump_fldata
+  (#k: parser_kind)
+  (#t: Type0)
+  (p: parser k t)
+  (sz: SZ.t)
+: LPS.jumper #t #(parse_fldata_kind (SZ.v sz) k) (parse_fldata p (SZ.v sz))
+=
+  (input: slice byte)
+  (offset: SZ.t)
+  (#pm: perm)
+  (#v: Ghost.erased bytes)
+{
+  parser_kind_prop_equiv (parse_fldata_kind (SZ.v sz) k) (parse_fldata p (SZ.v sz));
+  pts_to_len input;
+  SZ.add offset sz
+}
