src/lowparse/pulse/LowParse.PulseParse.List.fst
@@ -1,0 +1,76 @@
+module LowParse.PulseParse.List
+#lang-pulse
+include LowParse.Spec.List
+open FStar.Tactics.V2
+open Pulse.Lib.Pervasives open Pulse.Lib.Slice.Util open Pulse.Lib.Trade
+open Pulse.Lib.Slice
+open LowParse.Spec.Base
+
+module SZ = FStar.SizeT
+module R = Pulse.Lib.Reference
+module Trade = Pulse.Lib.Trade.Util
+module S = Pulse.Lib.Slice
+module LPS = LowParse.Pulse.Base
+
+let parse_consume (#k: parser_kind) (#t: Type) (p: parser k t) (b: bytes)
+: GTot (option nat)
+= match parse p b with
+  | Some (_, consumed) -> Some consumed
+  | None -> None
+
+inline_for_extraction
+fn validate_list
+  (#k: parser_kind)
+  (#t: Type0)
+  (#p: parser k t)
+  (v: LPS.validator p)
+  (u: squash (
+    k.parser_kind_subkind == Some ParserStrong /\
+    k.parser_kind_low > 0
+  ))
+: LPS.validator #(list t) #(parse_list_kind k.parser_kind_injective) (parse_list p)
+=
+  (input: slice byte)
+  (poffset: R.ref SZ.t)
+  (#offset: Ghost.erased SZ.t)
+  (#pm: perm)
+  (#v_bytes: Ghost.erased bytes)
+{
+  pts_to_len input;
+  parser_kind_prop_equiv k p;
+  let input_len = len input;
+  let mut pcontinue = true;
+  while (
+    let c = !pcontinue;
+    let off = !poffset;
+    (c && SZ.lt off input_len)
+  ) invariant exists* c off .
+    R.pts_to pcontinue c **
+    R.pts_to poffset off **
+    pts_to input #pm v_bytes **
+    pure (
+      SZ.v off <= Seq.length v_bytes /\
+      (c == true ==>
+        (Some? (parse (parse_list p) (Seq.slice v_bytes (SZ.v offset) (Seq.length v_bytes))) ==
+         Some? (parse (parse_list p) (Seq.slice v_bytes (SZ.v off) (Seq.length v_bytes))))) /\
+      (c == false ==> None? (parse (parse_list p) (Seq.slice v_bytes (SZ.v offset) (Seq.length v_bytes))))
+    )
+  {
+    let off = !poffset;
+    let s = Ghost.hide (Seq.slice v_bytes (SZ.v off) (Seq.length v_bytes));
+    parse_list_eq' p s;
+    let is_valid = v input poffset;
+    if (not is_valid) {
+      pcontinue := false
+    }
+  };
+  let off = !poffset;
+  let c = !pcontinue;
+  if c {
+    parse_list_eq p (Seq.slice v_bytes (SZ.v off) (Seq.length v_bytes));
+    parser_kind_prop_equiv (parse_list_kind k.parser_kind_injective) (parse_list p);
+    true
+  } else {
+    false
+  }
+}
