src/lowparse/pulse/LowParse.PulseParse.Option.fst
@@ -1,0 +1,37 @@
+module LowParse.PulseParse.Option
+#lang-pulse
+include LowParse.Spec.Option
+open FStar.Tactics.V2
+open Pulse.Lib.Pervasives open Pulse.Lib.Slice.Util open Pulse.Lib.Trade
+open Pulse.Lib.Slice
+open LowParse.Spec.Base
+
+module SZ = FStar.SizeT
+module R = Pulse.Lib.Reference
+module Trade = Pulse.Lib.Trade.Util
+module S = Pulse.Lib.Slice
+module LPS = LowParse.Pulse.Base
+
+inline_for_extraction
+fn validate_option
+  (#k: parser_kind)
+  (#t: Type0)
+  (#p: parser k t)
+  (v: LPS.validator p)
+: LPS.validator #(option t) #(parse_option_kind k) (parse_option p)
+=
+  (input: slice byte)
+  (poffset: R.ref SZ.t)
+  (#offset: Ghost.erased SZ.t)
+  (#pm: perm)
+  (#v_bytes: Ghost.erased bytes)
+{
+  let offset_val = !poffset;
+  let is_valid = v input poffset;
+  if is_valid {
+    true
+  } else {
+    poffset := offset_val;
+    true
+  }
+}
