src/lowparse/pulse/LowParse.PulseParse.VLData.fst
@@ -1,0 +1,136 @@
+module LowParse.PulseParse.VLData
+#lang-pulse
+include LowParse.Spec.VLData
+open FStar.Tactics.V2
+open Pulse.Lib.Pervasives open Pulse.Lib.Slice.Util open Pulse.Lib.Trade
+open Pulse.Lib.Slice
+open LowParse.Spec.Base
+
+module SZ = FStar.SizeT
+module R = Pulse.Lib.Reference
+module Trade = Pulse.Lib.Trade.Util
+module S = Pulse.Lib.Slice
+module LPS = LowParse.Pulse.Base
+module PPB = LowParse.PulseParse.Base
+module PPC = LowParse.PulseParse.Combinators
+module PPCF = LowParse.PulseParse.FLData
+module U32 = FStar.UInt32
+
+(* validate_vldata_gen: validate variable-length data with a bounded integer length prefix *)
+
+#push-options "--z3rlimit 32"
+
+inline_for_extraction
+fn validate_vldata_gen
+  (sz: integer_size)
+  (f: (bounded_integer sz -> GTot bool))
+  (f': (x: bounded_integer sz) -> (y: bool { y == f x }))
+  (#k: parser_kind)
+  (#t: Type0)
+  (#p: parser k t)
+  (v: LPS.validator p)
+  (lr: PPB.leaf_reader (parse_bounded_integer sz))
+  (u: squash FStar.SizeT.fits_u64)
+: LPS.validator #t #(parse_vldata_gen_kind sz k) (parse_vldata_gen sz f p)
+=
+  (input: slice byte)
+  (poffset: R.ref SZ.t)
+  (#offset: Ghost.erased SZ.t)
+  (#pm: perm)
+  (#v_bytes: Ghost.erased bytes)
+{
+  let sinput = Ghost.hide (Seq.slice v_bytes (SZ.v offset) (Seq.length v_bytes));
+  parse_vldata_gen_eq sz f p sinput;
+  parser_kind_prop_equiv (parse_bounded_integer_kind sz) (parse_bounded_integer sz);
+  pts_to_len input;
+  let offset_val = !poffset;
+  SZ.fits_u64_implies_fits_32 ();
+  let sz_sz = SZ.uint32_to_sizet (U32.uint_to_t sz);
+  let input_len = len input;
+  let remaining = SZ.sub input_len offset_val;
+  if SZ.lt remaining sz_sz {
+    false
+  } else {
+    LPS.validate_total_constant_size (parse_bounded_integer sz) sz_sz input poffset;
+    let off1 = !poffset;
+    let bi = PPB.read_parsed_from_validator_success lr input offset_val off1;
+    if not (f' bi) {
+      false
+    } else {
+      let len_payload = SZ.uint32_to_sizet bi;
+      let remaining2 = SZ.sub input_len off1;
+      if SZ.lt remaining2 len_payload {
+        false
+      } else {
+        let payload_end = SZ.add off1 len_payload;
+        let input3, input4 = split_trade input payload_end;
+        with v4 . assert (pts_to input4 #pm v4);
+        Trade.elim_hyp_r (pts_to input3 #pm _) (pts_to input4 #pm v4) (pts_to input #pm v_bytes);
+        poffset := off1;
+        let is_valid = v input3 poffset;
+        if is_valid {
+          let off2 = !poffset;
+          Trade.elim (pts_to input3 #pm _) (pts_to input #pm v_bytes);
+          if (off2 = payload_end) {
+            true
+          } else {
+            false
+          }
+        } else {
+          Trade.elim (pts_to input3 #pm _) (pts_to input #pm v_bytes);
+          false
+        }
+      }
+    }
+  }
+}
+
+#pop-options
+
+(* validate_bounded_vldata': bounded variable-length data *)
+
+inline_for_extraction
+fn validate_bounded_vldata'
+  (min: nat)
+  (max: nat { min <= max /\ max > 0 /\ max < 4294967296 })
+  (l: nat { l >= log256' max /\ l <= 4 })
+  (#k: parser_kind)
+  (#t: Type0)
+  (#p: parser k t)
+  (v: LPS.validator p)
+  (lr: PPB.leaf_reader (parse_bounded_integer l))
+  (u: squash FStar.SizeT.fits_u64)
+: LPS.validator #t #(parse_bounded_vldata_strong_kind min max l k) (parse_bounded_vldata' min max l p)
+=
+  (input: slice byte)
+  (poffset: R.ref SZ.t)
+  (#offset: Ghost.erased SZ.t)
+  (#pm: perm)
+  (#v_bytes: Ghost.erased bytes)
+{
+  parse_bounded_vldata_correct min max l p;
+  validate_vldata_gen l (in_bounds min max) (fun (i: bounded_integer l) -> if min = 0 then U32.lte i (U32.uint_to_t max) else (U32.lte (U32.uint_to_t min) i && U32.lte i (U32.uint_to_t max))) v lr () input poffset
+}
+
+(* validate_bounded_vldata: bounded variable-length data with default log *)
+
+inline_for_extraction
+fn validate_bounded_vldata
+  (min: nat)
+  (max: nat { min <= max /\ max > 0 /\ max < 4294967296 })
+  (#k: parser_kind)
+  (#t: Type0)
+  (#p: parser k t)
+  (v: LPS.validator p)
+  (lr: PPB.leaf_reader (parse_bounded_integer (log256' max)))
+  (u: squash FStar.SizeT.fits_u64)
+: LPS.validator #t #(parse_bounded_vldata_strong_kind min max (log256' max) k) (parse_bounded_vldata min max p)
+=
+  (input: slice byte)
+  (poffset: R.ref SZ.t)
+  (#offset: Ghost.erased SZ.t)
+  (#pm: perm)
+  (#v_bytes: Ghost.erased bytes)
+{
+  validate_bounded_vldata' min max (log256' max) v lr () input poffset
+}
